Single coin example

single_coin/SingleCoinA.v
@@ -1,33 +1,32 @@
 Require Import CRIS.
 Require Import SingleCoinHeader.
+Require Import ProphecyRA.
 From iris Require Import gmap_view.
 
-Section RA.
-  Context `{!crisG Γ Σ α β τ _I _S}.
-
-  Local Definition CoinRA : ucmra := gmap_viewUR nat (agreeR boolO).
-  Class coinG `{!crisG Γ Σ α β τ _I _S} := {
-      coin_inG :: inG CoinRA Γ
-  }.
-  Definition coinΓ : HRA := #[CoinRA].
-  Global Instance subG_coinG : subG coinΓ Γ → coinG.
-  Proof. solve_inG. Defined.
-End RA.
-Hint Unfold subG_coinG coin_inG : GRA_index.
+Local Definition CoinRA : ucmra := gmap_viewUR nat (agreeR boolO).
+Class coinGpreS `{!crisG Γ Σ α β τ _I _S} := {
+  #[local] coin_inG :: inG CoinRA Γ
+}.
+Class coinGS `{!crisG Γ Σ α β τ _I _S} := {
+  #[local] coinGS_coinGpreS :: coinGpreS;
+  coin_name : gname;
+}.
+Definition coinΓ : HRA := #[CoinRA].
+Global Instance subG_coinGpreS `{!crisG Γ Σ α β τ _I _S} : subG coinΓ Γ → coinGpreS.
+Proof. solve_inG. Defined.
 
 Section definitions.
-  Context `{_sinvG: !crisG Γ Σ α β τ _I _S}.
-  Context `{_coinG: !coinG}.
-  
+  Context `{!crisG Γ Σ α β τ _S _I, !concGS, !coinGS}.
+
   Definition coin_auth_r (l : list bool) : CoinRA :=
     gmap_view_auth (DfracOwn 1)
       (list_to_map (zip_with (λ a b, (a, b)) (seq 0 (length l)) (map (λ b, to_agree b) l))).
-  Definition coin_auth l : iProp Σ := own base_γ (coin_auth_r l).
+  Definition coin_auth l : iProp Σ := own coin_name (coin_auth_r l).
 
   Definition coin_r (n : nat) (b : bool) : CoinRA :=
     gmap_view_frag n (DfracOwn 1) (to_agree b).
   Definition coin (n : nat) (b : bool) : iProp Σ :=
-    own base_γ (coin_r n b).
+    own coin_name (coin_r n b).
 
   Lemma coin_alloc l b : coin_auth l ==∗ coin_auth (l ++ [b]) ∗ coin (length l) b.
   Proof.
@@ -51,7 +50,7 @@ Section definitions.
     { ss. }
   Qed.
 
-  Lemma coin_both_valid l n b : coin_auth l -∗ coin n b -∗ ⌜nth_error l n = Some b⌝.
+  Lemma coin_both_valid l n b : coin_auth l -∗ coin n b -∗ ⌜l !! n = Some b⌝.
   Proof.
     iIntros "A C"; iCombine "A" "C" gives %WF.
     rewrite /coin_auth_r /coin_r in WF.
@@ -59,19 +58,18 @@ Section definitions.
     eapply elem_of_list_to_map in EQ; cycle 1.
     { rewrite fst_zip; [|rewrite length_map length_seq //]. apply NoDup_seq. }
     apply elem_of_lookup_zip_with in EQ; destruct EQ as [? [? [? [EQ ?]]]]; clarify.
-    des. apply lookup_seq in H1; des; clarify; ss.
-    apply Some_pair_included_r in H2. rewrite Some_included_total in H2.
-    apply elem_of_list_split_length in H3. destruct H3 as [l1 [l2 [EQ EQL]]].
+    des. apply lookup_seq in H3; des; clarify; ss.
+    apply Some_pair_included_r in H4. rewrite Some_included_total in H4.
+    apply elem_of_list_split_length in H5. destruct H5 as [l1 [l2 [EQ EQL]]].
     apply map_eq_app in EQ; destruct EQ as [l1' [l2' [-> [EQ1 EQ2]]]].
     destruct l2'; [inv EQ2|ss]. inv EQ2.
-    apply to_agree_included in H2; inv H2.
-    rewrite length_map. rewrite nth_error_app2 // Nat.sub_diag //.
+    apply to_agree_included in H4; inv H4.
+    rewrite length_map. rewrite lookup_app_r // Nat.sub_diag //.
   Qed.
 End definitions.
 
-Module SingleCoinAS. Section SingleCoinAS.
-  Context `{_crisG: !crisG Γ Σ α β τ _I _S}.
-  Context `{_coinG: !coinG}.
+Module SingleCoinA. Section SingleCoinA.
+  Context `{!crisG Γ Σ α β τ _S _I, !concGS, !coinGS, !prophGS}.
 
   Definition new_spec : fspec :=
     fspec_simple (λ _ : unit,
@@ -85,32 +83,22 @@ Module SingleCoinAS. Section SingleCoinAS.
       (λ vret, ⌜vret = b↑⌝ ∗ coin n b))
     )%I.
 
-  Definition sp : alist string fspec :=
-    Seal.sealing CRIS
-      [(SingleCoinHdr.new, new_spec);
-       (SingleCoinHdr.read, read_spec)
-      ].
-End SingleCoinAS. End SingleCoinAS.
-
-Module SingleCoinA. Section SingleCoinA.
-  Context `{_crisG: !crisG Γ Σ α β τ _I _S}.
-  Context `{_coinG: !coinG}.
-  Import SingleCoinAS.
-
   Definition scopes : list string := [].
 
-  Definition fnsems : fnsems_type :=
-    [(Some SingleCoinHdr.new, (true, wmask_all, scopes, (fsp_some new_spec, fbody_trivial)));
-     (Some SingleCoinHdr.read, (true, wmask_all, scopes, (fsp_some read_spec, fbody_trivial)))
-    ].
+  Definition fnsems : fnsemmap :=
+    {[Some SingleCoinHdr.new := Some (msk_scp scopes msk_true, (fsp_some new_spec, fbody_trivial));
+      Some SingleCoinHdr.read := Some (msk_scp scopes msk_true, (fsp_some read_spec, fbody_trivial))]}.
 
   Program Definition Mod : SMod.t := {|
     SMod.scopes := scopes;
     SMod.fnsems := fnsems;
-    SMod.initial_st := [];
+    SMod.initial_st := ∅;
   |}.
-  Solve All Obligations with prove_scope.
-  Next Obligation. prove_nodup. Qed.
+  Solve All Obligations with mod_tac.
 
-  Definition t sp : Mod.t := Seal.sealing CRIS (SMod.to_mod sp Mod).
+  Definition init_cond : iProp Σ :=
+    coin_auth nil ∗
+    ProphecyRA.free_id (λ i, i.1 = "SingleCoin" ∧ ∃ n, i.2↓↓ = Some n ∧ n >= 0)%type.
+
+  Definition t sp : Mod.t := SMod.to_mod sp Mod.
 End SingleCoinA. End SingleCoinA.
