single_coin/SingleCoinPAproof.v
@@ -1,6 +1,6 @@
 Require Import CRIS.
-Require Import SingleCoinHeader SingleCoinP SingleCoinA.
-Require Import ProphecyHeader ProphecyA.
+Require Export SingleCoinHeader SingleCoinP SingleCoinA.
+Require Export ProphecyHeader ProphecyA.
 
 Local Program Definition coin_proph : Prophecy.t := {|
   Prophecy.Pro := bool;
@@ -18,451 +18,129 @@ Next Obligation.
 Qed.
 
 Module SingleCoinPA. Section SingleCoinPA.
-  Import SingleCoinAS SingleCoinP.
-  Context `{_crisG: !crisG Γ Σ α β τ _I _S}.
-  Context `{_prophG: !prophG}.
-  Context `{_coinG: !coinG}.
+  Import SingleCoinA SingleCoinP.
+  Context `{!crisG Γ Σ α β τ _S _I, !concGS, !prophGS, !coinGS}.
+  Context (mn : string) (sp : specmap).
 
-  Context (sp : sp_type).
+  Local Notation MA := (SingleCoinA.t sp).
+  Local Notation MI := (SingleCoinP.t mn ★ ProphecyA.t mn ∅).
 
-  Local Definition MA := SingleCoinA.t sp.
-  Local Definition MI := SingleCoinP.t ★ ProphecyA.t sp.
-
-  Local Definition Ist : alist key Any.t → alist key Any.t → iProp Σ :=
+  Local Definition Ist : ist_type Σ :=
     (λ st_s st_t,
       ∃ (l_s : list bool) (l_t : list (option bool)),
-        ⌜st_s = [] ∧ st_t = [(v_coins, l_t↑)] ∧ length l_s = length l_t⌝
+        ⌜st_t = {[v_coins := Some l_t↑]} ∧ length l_s = length l_t⌝
         ∗ ProphecyRA.free_id (λ i, i.1 = "SingleCoin" ∧ ∃ n, i.2↓↓ = Some n ∧ n >= length l_t)%type
         ∗ coin_auth l_s
         ∗ [∗ list] i ↦ ob ∈ l_t,
           ∃ b ol, ProphecyRA.has_proph (proph_coins i) (existT coin_proph (b, ol))
-          ∗ ⌜nth_error l_s i = Some b
+          ∗ ⌜l_s !! i = Some b
             ∧ (match ob with Some b' => b' = b ∧ ol = [b] | None => ol = [] end)
             ∧ (Prophecy.consistent coin_proph ol b)⌝
         )%I.
 
-  (* Lemma simF_new : HSim.sim_fun open MA MI Ist SingleCoinHdr.new. *)
-  (* Proof. *)
-  (*   init_simF. *)
+  Lemma simF_new : ISim.sim_fun open MA MI Ist (Some SingleCoinHdr.new).
+  Proof.
+    iStartSim.
+    iDestruct "IST" as (l_s l_t) "[[-> %EQ] [F [AUTH PL]]]".
+    steps_l. iDestruct "ASM" as "[-> ->]". hss.
 
-  (*   iDestruct "IST" as (l_s l_t) "[[-> [-> %EQ]] [F [AUTH PL]]]". *)
+    steps_r. inline_r. force_r (proph_coins (length l_t), coin_proph).
+    steps_r. force_r ((proph_coins (length l_t))↑). steps_r.
+    iPoseProof (ProphecyRA.free_id_split _ (proph_coins (length l_t)) with "F") as "> [F1 F2]".
+    { ss; hss; esplits; eauto. }
+    force_r; iFrame; iSplit; eauto.
+    steps_r. iDestruct "GRT" as "[-> [%b [-> P]]]". steps_r.
 
-  (*   steps_l. iDestruct "ASM" as "[-> ->]". hss. *)
+    (* alloc coin *)
+    iMod (coin_alloc _ b with "AUTH") as "[AUTH COIN]".
+    iIst "IST" with "[F2 PL P AUTH]".
+    { iExists (l_s ++ [b]), (l_t ++ [None]). iSplit; eauto.
+      { iPureIntro; splits; ss; eauto. rewrite ?length_app; s; lia. }
+      iSplitL "F2".
+      { iApply ProphecyRA.free_id_iff; [|iFrame].
+        intros [name a]; split; ss; des_ifs.
+        { intros t; inv t; des; clarify. inv e. hss. rewrite length_app in H3. ss. lia. }
+        { intros t; des; esplits; eauto. rewrite length_app in t1; ss; lia. }
+        { intros [-> [n0 [EQ' GT]]]; esplits; eauto.
+          assert (n0 <> length l_t).
+          { ii; clarify; eapply n; rewrite /proph_coins; f_equal. hexploit SAny.downcast_upcast; eauto. }
+          rewrite length_app; ss; lia.
+        }
+      }
+      iFrame.
+      iApply (big_sepL_app). iSplitL "PL"; cycle 1.
+      { s. iSplit; [|done]. iExists b, []; iSplit.
+        { rewrite Nat.add_0_r; iFrame. }
+        iPureIntro. rewrite -EQ.
+        rewrite lookup_app_r; [|lia].
+        rewrite Nat.add_comm /= Nat.sub_diag /=.
+        esplits; eauto.
+      }
+      iApply (big_sepL_impl with "PL").
+      iModIntro; iIntros (k x) "% [%b' [%ol' H]]".
+      apply lookup_lt_Some in H3; rewrite -EQ in H3.
+      rewrite lookup_app_l //.
+      iExists _, _; iFrame.
+    }
 
-  (*   steps_r. hss. steps_r. hss. *)
-  (*   inline_r. force_r (proph_coins (length l_t), coin_proph). steps_r. *)
-  (*   force_r ((proph_coins (length l_t))↑). steps_r. *)
-  (*   iPoseProof (ProphecyAS.free_id_split _ (proph_coins (length l_t)) with "F") as "> [F1 F2]". *)
-  (*   { ss; hss; esplits; eauto. } *)
-  (*   force_r; iFrame; iSplit; eauto. *)
-  (*   steps_r. iDestruct "GRT" as "[[%b [-> P]] ->]". hss. steps_r. *)
-  (*   (* alloc coin *) *)
-  (*   iMod (coin_alloc _ b with "AUTH") as "[AUTH COIN]". *)
+    forces_l. iFrame. iSplit; eauto.
+    step. iFrame. eauto.
+  Qed.
 
-  (*   iAssert (Ist nths [] [(v_coins, (l_t ++ [None])↑)]) with "[F2 PL P AUTH]" as "IST". *)
-  (*   { rewrite /Ist /=. iExists (l_s ++ [b]), (l_t ++ [None]). iSplit; eauto. *)
-  (*     { iPureIntro; splits; ss; eauto. rewrite ?length_app; s; lia. } *)
-  (*     iSplitL "F2". *)
-  (*     { iApply ProphecyAS.free_id_iff; [|iFrame]. *)
-  (*       intros [name a]; split; ss; des_ifs. *)
-  (*       { intros H; inv H; des; clarify. inv e. hss. rewrite length_app in H0. ss. lia. } *)
-  (*       { intros H; des; esplits; eauto. rewrite length_app in H1; ss; lia. } *)
-  (*       { intros [-> [n0 [EQ' GT]]]; esplits; eauto. *)
-  (*         assert (n0 <> length l_t). *)
-  (*         { ii; clarify; eapply n; rewrite /proph_coins; f_equal. hexploit SAny.downcast_upcast; eauto. } *)
-  (*         rewrite length_app; ss; lia. *)
-  (*       } *)
-  (*     } *)
-  (*     iFrame. *)
-  (*     iApply (big_sepL_app). iSplitL "PL"; cycle 1. *)
-  (*     { s. iSplit; [|done]. iExists b, []; iSplit. *)
-  (*       { rewrite Nat.add_0_r; iFrame. } *)
-  (*       iPureIntro. rewrite -EQ. rewrite nth_error_app2; rewrite Nat.add_0_r // Nat.sub_diag /=. *)
-  (*       splits; ss. *)
-  (*       eauto. *)
-  (*     } *)
-  (*     iApply (big_sepL_impl with "PL"). *)
-  (*     iModIntro; iIntros (k x) "% [%b' [%ol' H]]". *)
-  (*     apply lookup_lt_Some in H; rewrite -EQ in H. rewrite nth_error_app1 //. *)
-  (*     iExists _, _; iFrame. *)
-  (*   } *)
+  Lemma simF_read : ISim.sim_fun open MA MI Ist (Some SingleCoinHdr.read).
+  Proof.
+    iStartSim.
+    steps_l. destruct _q as [idx b]. iDestruct "ASM" as "[-> [-> C]]".
+    iDestruct "IST" as (l_s l_t) "[[-> %EQ] [F [AU PL]]]".
+    iPoseProof (coin_both_valid with "AU C") as "%NTH".
 
-  (*   forces_l. iFrame. iSplit; eauto. *)
-  (*   steps_l. step. iFrame. rewrite EQ; done. *)
-  (* Qed. *)
+    steps_r.
+    assert (idx < length l_s) by (eapply lookup_lt_Some; eauto).
+    destruct (l_t !! idx) as [o|] eqn : LTN; cycle 1.
+    { apply lookup_ge_None in LTN; lia. }
+    destruct o as [bn'|].
+    { (* after initialization *)
+      iPoseProof (big_sepL_lookup_acc _ _ idx with "PL") as "[P PL]"; eauto.
+      iDestruct "P" as "[%bn [%oln [P %P]]]".
+      rewrite NTH in P. rewrite NTH. destruct P as [NTH' [EQ' ?]].
+      hexploit EQ'; ss; i; des; clarify.
+      forces_l. iFrame. iSplit; eauto.
+      step. iSplit; eauto.
+      iFrame. iSplit; eauto. iApply "PL". iExists _, _; iFrame.
+      iPureIntro; splits; ss. right; esplits; eauto.
+    }
+    { (* before initialization *)
+      eapply elem_of_list_split_length in LTN; destruct LTN as [l1 [l2 [-> ->]]].
+      steps_r. rewrite take_app Nat.sub_diag /= app_nil_r firstn_all drop_app.
+      rewrite drop_ge; [|lia]; rewrite /= Nat.sub_succ_l // Nat.sub_diag /= drop_0.
+      iPoseProof (big_sepL_app with "PL") as "[PL1 [P PL2]]".
+      iDestruct "P" as "[%bn [%oln [P %HP]]]".
+      inline_r. force_r (proph_coins _, existT coin_proph (_, _, _)). forces_r. iFrame.
+      rewrite Nat.add_0_r. iSplit; eauto.
+      steps_r. iDestruct "GRT" as "[-> [[-> %GRT] P]]". steps_r.
+      destruct GRT as [|[tl EQ']]; [clarify|].
+      destruct tl; cycle 1.
+      { inv EQ'. destruct HP as [? [Htemp ?]]. exfalso; eapply app_cons_not_nil; eauto. }
+      inv EQ'.
 
-  (* Lemma simF_read : HSim.sim_fun open MA MI Ist SingleCoinHdr.read. *)
-  (* Proof. *)
-  (*   init_simF. *)
-  (*   steps_l. iDestruct "ASM" as "[[-> C] ->]". hss. rename q1 into n, q2 into b. *)
-  (*   iDestruct "IST" as (l_s l_t) "[[-> [-> %EQ]] [F [AU PL]]]". *)
-  (*   iPoseProof (coin_both_valid with "AU C") as "%NTH". *)
+      forces_l. iFrame. iSplit; eauto. step.
+      rewrite Nat.add_0_r NTH in HP; destruct HP as [? [_ HP]]; clarify.
+      iSplit; eauto.
+      iExists l_s, _. iSplit; [iPureIntro; splits; eauto|].
+      { rewrite EQ ?length_app /= //. }
+      iSplitL "F".
+      { iApply ProphecyRA.free_id_iff; ss. rewrite ?length_app //. }
+      iFrame.
+      iExists bn, [bn]; rewrite Nat.add_0_r. iFrame.
+      iPureIntro; ss; esplits; eauto. right; exists []; eauto.
+    }
+  Qed.
 
-  (*   steps_r. hss. steps_r. *)
-  (*   assert (n < length l_s) by (apply nth_error_Some; ii; clarify). *)
-  (*   destruct (nth_error l_t n) eqn : LTN; cycle 1. *)
-  (*   { apply nth_error_None in LTN. lia. } *)
-  (*   destruct o as [bn'|]. *)
-  (*   { (* after initialization *) *)
-  (*     iPoseProof (big_sepL_lookup_acc _ _ n with "PL") as "[P PL]". *)
-  (*     { edestruct (nth_lookup_or_length l_t n); eauto. lia. } *)
-  (*     iDestruct "P" as "[%bn [%oln [P %P]]]". *)
-  (*     eapply nth_error_nth in LTN. rewrite LTN in P. rewrite LTN. destruct P as [NTH' [EQ' ?]]. *)
-  (*     hexploit EQ'; ss; i; des; clarify. *)
-  (*     forces_l. iFrame. iSplit; eauto. *)
-  (*     steps_l. steps_r. step. iSplit; eauto. *)
-  (*     iFrame. iSplit; eauto. iApply "PL". iExists _, _; iFrame. rewrite NTH'. *)
-  (*     iPureIntro; splits; ss. right; esplits; eauto. *)
-  (*   } *)
-  (*   { (* before initialization *) *)
-  (*     hexploit nth_error_split; eauto. *)
-  (*     intros [lt_1 [lt_2 [-> LEN1]]]. *)
-  (*     steps_r. rewrite take_app Nat.sub_diag /= app_nil_r firstn_all drop_app. *)
-  (*     rewrite drop_ge; [|lia]; rewrite /= Nat.sub_succ_l // Nat.sub_diag /= drop_0. *)
-  (*     iPoseProof (big_sepL_app with "PL") as "[PL1 [P PL2]]". *)
-  (*     iDestruct "P" as "[%bn [%oln [P %HP]]]". *)
-  (*     inline_r. force_r (proph_coins _, existT coin_proph (_, _, _)). forces_r. iFrame. *)
-  (*     rewrite Nat.add_0_r. iSplit; eauto. *)
-  (*     steps_r. iDestruct "GRT" as "[[[-> %GRT] P] ->]". hss. *)
-  (*     destruct GRT as [|[tl EQ']]; [clarify|]. *)
-  (*     destruct tl; cycle 1. *)
-  (*     { inv EQ'. eapply app_cons_not_nil in H2; ss. } *)
-  (*     inv EQ'. *)
-
-  (*     steps_r. *)
-  (*     forces_l. iFrame. iSplit; eauto. steps_l. step. *)
-  (*     rewrite Nat.add_0_r in HP; clarify. *)
-  (*     iSplit; eauto. *)
-  (*     iExists l_s, _. iSplit; [iPureIntro; splits; eauto|]. *)
-  (*     { rewrite EQ ?length_app /= //. } *)
-  (*     iSplitL "F". *)
-  (*     { iApply ProphecyAS.free_id_iff; ss. rewrite ?length_app //. } *)
-  (*     iFrame. *)
-  (*     iExists b, [b]; rewrite Nat.add_0_r. iFrame. *)
-  (*     iPureIntro; ss; esplits; eauto. right; exists []; eauto. *)
-  (*   } *)
-  (*   Unshelve. all: exact None. *)
-  (* Qed. *)
-
-  (* Theorem sim : HSim.t MA MI ? IstFull.
+  Lemma sim : ISim.t open MA MI SingleCoinA.init_cond Ist.
   Proof.
     init_sim.
-    - iIntros "A". iExists _,_,[],[]. iSplit.
-      { rewrite !app_nil_r. eauto. }
-      iSplit; [iSplit|]; eauto. iExists _,_. iSplit; et.
-    - eapply simF_new; eauto.
-    - eapply simF_read; eauto.
-  Qed. *)
+    { iIntros "[A F]". iExists [], []. iSplit; eauto. iFrame. ss. }
+    { eapply simF_new; eauto. }
+    { eapply simF_read; eauto. }
+  Qed.
 End SingleCoinPA. End SingleCoinPA.
-
-(* Require Import Coqlib ITreelib sflib.
-Require Import SingleCoinHeader SingleCoinP SingleCoinA SingleCoinASpec SMod ModSim.
-Require Import Any Skeleton.
-Require Import PCM IPM.
-Require Import Events Behavior.
-Require Import ProphecyHeader ProphecyA STB.
-
-Require Import ISim HMod PMod Events ITactics.
-Require Import Mod ModSimFacts.
-
-Require Import sProp sWorld World SRF.
-Require Import Ensembles.
-
-Set Implicit Arguments.
-
-Local Open Scope nat_scope.
-
-Module SingleCoinPA.
-Section SIMMODSEM.
-  Context `{_W: CtxWD.t}.
-  Context `{_S: SingleCoinAR.t (Γ:=Γ)}.
-  Context `{_M: ProphecyAR.t (Γ:=Γ)}.
-
-  Fixpoint initialized_until (l_tgt : list (option bool)) (l_src: list bool) (hi: nat) : iProp :=
-    match hi with
-    | S hi' =>
-        SingleCoinAS.readable hi' ∗
-        (⌜exists b, nth_error l_tgt hi' = Some (Some b) /\ nth_error l_src hi' = Some b⌝
-         ∨
-         (∃ (b : bool) nth,
-          ProphecyAS.has_proph ("SingleCoin", hi'↑↑) (existT SingleCoinPrT.t (Full_set _, b, nth))
-            ∗ ⌜nth_error l_src hi' = Some b /\ nth_error l_tgt hi' = Some None⌝))
-        ∗ initialized_until l_tgt l_src hi'
-    | O => emp%I
-    end.
-
-  Lemma free_from_split i:
-    SingleCoinAS.free_from i -∗ SingleCoinAS.free_from (S i) ∗ (ProphecyAS.free_id (SingleCoinP.proph_coins i)).
-  Proof.
-    iIntros "H". unfold SingleCoinAS.free_from, ProphecyAS.free_id.
-    replace (SingleCoinAS.free_from_r i) with (SingleCoinAS.free_from_r (S i) ⋅ ProphecyAS.free_id_r (SingleCoinP.proph_coins i)).
-    { iDestruct "H" as "($ & $)". }
-    unfold SingleCoinAS.free_from_r, ProphecyAS.free_id_r. ur. unfold Auth.white. f_equal.
-    unfold SingleCoinAS.SingleCoinFree_r. ur. extensionalities.
-    unfold SingleCoinP.proph_coins. des_ifs; try solve [ur; des_ifs]; try nia.
-    - rewrite SAny.upcast_downcast in Heq. clarify. nia.
-    - rewrite SAny.upcast_downcast in Heq. clarify.
-    - exfalso. apply n1. f_equal. apply SAny.downcast_upcast. rewrite Heq. f_equal.
-      nia.
-    - rewrite SAny.upcast_downcast in Heq. clarify.
-  Qed.
-
-  Lemma uninitialized_from_split i:
-    SingleCoinAS.uninitialized_from i -∗ SingleCoinAS.uninitialized_from (S i) ∗ (SingleCoinAS.uninitialized i).
-  Proof.
-    iIntros "H". unfold SingleCoinAS.uninitialized_from, SingleCoinAS.uninitialized.
-    replace (SingleCoinAS.uninitialized_from_r i) with (SingleCoinAS.uninitialized_from_r (S i) ⋅ SingleCoinAS.uninitialized_r i).
-    { iDestruct "H" as "($ & $)". }
-    unfold SingleCoinAS.uninitialized_from_r, SingleCoinAS.uninitialized_r. ur.
-    extensionalities. des_ifs; try nia; try solve [ur; des_ifs].
-  Qed.
-
-  Lemma update_to_readable l :
-    SingleCoinAS.uninitialized l ==∗ SingleCoinAS.readable l.
-  Proof.
-    iIntros "H". unfold SingleCoinAS.uninitialized, SingleCoinAS.readable.
-    iPoseProof (OwnM_Upd with "H") as "D"; et. ii. ur. ur in H2. i.
-    specialize (H2 k). unfold SingleCoinAS.uninitialized_r, SingleCoinAS.readable_r in *.
-    destruct dec; clarify. ur in H2. ur. des_ifs.
-  Qed.
-
-  Lemma uninitialized_from_update i:
-    SingleCoinAS.uninitialized_from i ==∗ SingleCoinAS.uninitialized_from (S i) ∗ (SingleCoinAS.readable i).
-  Proof.
-    iIntros "H". iPoseProof (uninitialized_from_split with "H") as "(H0 & H1)".
-    iPoseProof (update_to_readable with "H1") as "> H1". iModIntro. iFrame.
-  Qed.
-
-  Lemma initialized_until_readable l l0 i:
-    initialized_until l l0 (S i) -∗ initialized_until l l0 (S i) ∗ SingleCoinAS.readable i.
-  Proof.
-    iIntros "H". ss. unfold SingleCoinAS.readable. set (SingleCoinAS.readable_r i) at 1.
-    replace c with ((SingleCoinAS.readable_r i) ⋅ (SingleCoinAS.readable_r i)).
-    { iDestruct "H" as "(($ & $) & $ & $)". }
-    unfold c, SingleCoinAS.readable_r. ur. extensionalities. des_ifs; ur; des_ifs.
-  Qed.
-
-  Lemma _initialized_update l_tgt l_src i b (EQ : List.length l_tgt = List.length l_src) (LE : i ≤ List.length l_src):
-    initialized_until l_tgt l_src i
-      -∗ SingleCoinAS.uninitialized_from i
-      -∗ ProphecyAS.has_proph (SingleCoinP.proph_coins i) (existT SingleCoinPrT.t (Full_set bool, b, 0))
-      ==∗ initialized_until (firstn i l_tgt ++ [None] ++ skipn (S i) l_tgt) (firstn i l_src ++ [b] ++ skipn (S i) l_src) (S i) ∗ SingleCoinAS.uninitialized_from (S i).
-  Proof.
-    iIntros "H0 H1 H2". ss. iPoseProof (uninitialized_from_update with "H1") as ">[? ?]".
-    iModIntro. iFrame. iSplitL "H2".
-    - iRight. iExists _,_. iFrame. iPureIntro. rewrite !nth_error_app2.
-      2:{ rewrite take_length. nia. }
-      2:{ rewrite take_length. nia. }
-      rewrite !take_length. replace (i - _) with 0 by nia. replace (i - _) with 0 by nia.
-      ss.
-    - set i at 1 6. assert (LE0 : n ≤ i) by nia. clearbody n.
-      iInduction n as [|n'] "IH" forall (LE0); ss.
-      iDestruct "H0" as "(R & D & I)"; iFrame.
-      iSplitR "I". 2:{ iApply "IH"; et. iPureIntro. nia. }
-      iDestruct "D" as "[%yes|no]".
-      + des. iLeft. iPureIntro.
-        rewrite <- (take_drop i l_tgt) in yes.
-        rewrite <- (take_drop i l_src) in yes0.
-        rewrite !nth_error_app1 in *; try solve [rewrite take_length; nia]; et.
-      + iRight. iDestruct "no" as "(%b0 & %nth & P & %X)". iExists _,_. iFrame.
-        iPureIntro.
-        rewrite <- (take_drop i l_src) in X.
-        rewrite <- (take_drop i l_tgt) in X.
-        rewrite !nth_error_app1 in *; try solve [rewrite take_length; nia]; et.
-  Qed.
-
-  Lemma initialized_update l_tgt l_src b (EQ : List.length l_tgt = List.length l_src) :
-    initialized_until l_tgt l_src (List.length l_src)
-      -∗ SingleCoinAS.uninitialized_from (List.length l_src)
-      -∗ ProphecyAS.has_proph (SingleCoinP.proph_coins (List.length l_src)) (existT SingleCoinPrT.t (Full_set bool, b, 0))
-      ==∗ initialized_until (l_tgt ++ [None]) (l_src ++ [b]) (S (List.length l_src)) ∗ SingleCoinAS.uninitialized_from (S (List.length l_src)).
-  Proof.
-    eassert (l_tgt ++ [None] = _); cycle 1.
-    eassert (l_src ++ [b] = _); cycle 1. rewrite H2. rewrite H3.
-    apply _initialized_update; et.
-    - destruct (drop _ l_src) eqn:E; et.
-      2:{ apply (f_equal List.length) in E. rewrite drop_length in E. ss. nia. }
-      rewrite app_nil_r. f_equal. set l_src at 1.
-      rewrite <- (take_drop (List.length l_src) l). unfold l. clear l.
-      destruct (drop (List.length l_src) l_src) eqn:E0; et.
-      2:{ apply (f_equal List.length) in E0. rewrite drop_length in E0. ss. nia. }
-      rewrite app_nil_r. et.
-    - destruct (drop _ l_tgt) eqn:E; et.
-      2:{ apply (f_equal List.length) in E. rewrite drop_length in E. ss. nia. }
-      rewrite app_nil_r. f_equal. set l_tgt at 1.
-      rewrite <- (take_drop (List.length l_src) l). unfold l. clear l.
-      destruct (drop (List.length l_src) l_tgt) eqn:E0; et.
-      2:{ apply (f_equal List.length) in E0. rewrite drop_length in E0. ss. nia. }
-      rewrite app_nil_r. et.
-  Qed.
-
-  Lemma uninitialized_readable_disjoint i j:
-       SingleCoinAS.uninitialized_from i -∗ SingleCoinAS.readable j -∗ ⌜j < i⌝.
-  Proof.
-    iIntros "A B". unfold SingleCoinAS.uninitialized_from, SingleCoinAS.readable.
-    unfold SingleCoinAS.uninitialized_from_r, SingleCoinAS.readable_r.
-    destruct (le_dec i j). 2:{ iPureIntro. nia. }
-    iCombine "A B" as "C". iOwnWf "C" as wfc. exfalso.
-    ur in wfc. specialize (wfc j). des_ifs; try nia. ur in wfc. et.
-  Qed.
-
-  Lemma initialized_until_same i j l_src l_tgt b b0 (ran : i < j)
-    (E : nth_error l_src i = Some b) (E0 : nth_error l_tgt i = Some (Some b0)) :
-  initialized_until l_tgt l_src j -∗ ⌜b = b0⌝.
-  Proof.
-    iInduction j as [|j'] "IH"; try nia.
-    iIntros "H". destruct (dec i j'); cycle 1.
-    { ss. iDestruct "H" as "(_ & _ & H)". iApply "IH"; iFrame. iPureIntro. nia. }
-    clarify. ss. iDestruct "H" as "(_ & [%yes|no] & _)".
-    - des. rewrite E0 in yes. rewrite E in yes0. clarify.
-    - iDestruct "no" as "(%b1 & %nth & _ & %E1)". des. clarify.
-  Qed.
-
-  Lemma initialized_until_update_proph b i j l_src l_tgt (ran : i < j) 
-    (E : nth_error l_src i = Some b)
-    (E0 : nth_error l_tgt i = Some None) :
-  initialized_until l_tgt l_src j -∗
-  (initialized_until (take i l_tgt ++ Some b :: drop (S i) l_tgt) l_src j
-   ∗ ∃ nth, ProphecyAS.has_proph ("SingleCoin", i↑↑) (existT SingleCoinPrT.t (Full_set _, b, nth))).
-  Proof.
-    iInduction j as [|j'] "IH"; try nia.
-    iIntros "H". destruct (dec i j'); cycle 1.
-    - ss. iDestruct "H" as "(A & B & H)".
-      assert (X: i < j') by nia. iPoseProof ("IH" $! X with "H") as "[I P]". 
-      iFrame. iDestruct "B" as "[%yes|no]".
-      + des. iLeft. iPureIntro. rewrite yes0. esplits; et.
-        rewrite <- (take_drop (S i) l_tgt) in yes.
-        rewrite !nth_error_app2 in *. 2:{ rewrite take_length. nia. }
-        2:{ rewrite take_length. nia. }
-        rewrite take_length in *.
-        assert (i < List.length l_tgt).
-        { rewrite <- nth_error_Some. rewrite E0. et. }
-        replace (_ `min` _) with i by nia.
-        replace (_ `min` _) with (S i) in yes by nia.
-        change (Some b :: _) with ([Some b] ++ (drop (S i) l_tgt)).
-        rewrite nth_error_app2; ss. 2:{ nia. }
-        rewrite <- yes. f_equal. nia.
-      + iDestruct "no" as "(%b0 & %nth & P & %L)".
-        des. iRight. iExists _,_. iFrame. iPureIntro. split; et.
-        rewrite <- (take_drop (S i) l_tgt) in L0.
-        rewrite !nth_error_app2 in *; rewrite take_length in *; try nia.
-        assert (i < List.length l_tgt).
-        { rewrite <- nth_error_Some. rewrite E0. et. }
-        replace (_ `min` _) with i by nia.
-        replace (_ `min` _) with (S i) in L0 by nia.
-        change (Some b :: _) with ([Some b] ++ (drop (S i) l_tgt)).
-        rewrite nth_error_app2; ss. 2:{ nia. }
-        rewrite <- L0. f_equal. nia.
-    - clarify. ss. iDestruct "H" as "($ & [%yes|no] & I)". { des. clarify. }
-      iDestruct "no" as "(%b0 & %nth & P & %L)". des. iSplitR "P". 2:{ rewrite E in L. clarify. et. }
-                                                                 iSplitR.
-      + iLeft. iExists b0. iPureIntro. rewrite E in L. clarify. split; et.
-        rewrite nth_error_app2. 2:{ rewrite take_length. nia. }
-        rewrite take_length. 
-        assert (j' < List.length l_tgt).
-        { rewrite <- nth_error_Some. rewrite L0. et. }
-        replace (_ - _) with 0 by nia. ss.
-      + iClear "IH". set (take j' l_tgt ++ Some b :: drop (S j') l_tgt).
-        assert (j' < List.length l_tgt).
-        { rewrite <- nth_error_Some. rewrite L0. et. }
-        assert (forall i, i < j' -> nth_error l_tgt i = nth_error l i).
-        { i. unfold l. set l_tgt at 1. rewrite <- (take_drop j' l0).
-          unfold l0. rewrite !nth_error_app1; et.
-          all: try solve [rewrite take_length; nia]. }
-        clearbody l. clear - H3.
-        iInduction j' as [|j'] "IH" forall (H3); ss.
-        iDestruct "I" as "($ & H & I)". iSplitR "I". 2:{ iApply "IH"; et. }
-        iDestruct "H" as "[%yes|no]".
-        { iLeft. iPureIntro. des. esplits; et. rewrite <- H3; try nia. et. }
-        iRight. iDestruct "no" as "(%b0 & %nth & P & %L)". des.
-        iExists _,_. iFrame. iPureIntro. split; et. rewrite <- H3; et.
-   Qed.
-
-  Definition Ist: Sk.t -> nat -> alist key Any.t -> alist key Any.t -> iProp :=
-    (fun _ _ st_src st_tgt =>
-      ∃ l_tgt l_src,
-      ⌜st_tgt = [(SingleCoinP.v_coins, (l_tgt : list (option bool))↑)] /\
-       st_src = [(SingleCoinA.v_coins, (l_src : list bool)↑)] /\
-       List.length l_tgt = List.length l_src⌝ ∗
-      initialized_until l_tgt l_src (List.length l_src) ∗
-      SingleCoinAS.free_from (List.length l_src) ∗ SingleCoinAS.uninitialized_from (List.length l_src))%I.
-
-  Variable ginv: Sk.t -> invspec.
-  Variable StbProph: Sk.t -> gname -> option fspec.
-  Variable StbSingleCoin: Sk.t -> gname -> option fspec.
-
-  Local Notation ProphecyA := (ProphecyA.t ginv StbProph).
-  Local Notation SingleCoinA := (SingleCoinA.t ginv StbSingleCoin).
-  Local Notation SingleCoinAMod := (SingleCoinA ★ ProphecyA).
-  Local Notation SingleCoinPMod := (SingleCoinP.t ★ ProphecyA).
-  Local Notation IstFull := (IstProd (IstSB SingleCoinA Ist) IstEq).
-
-  (**********)
-
-  Lemma simF_new:
-    HSim.sim_fun SingleCoinAMod SingleCoinPMod IstFull SingleCoinName.new.
-  Proof.
-    init_simF. unfold IstFull, IstProd0.
-    iDestruct "IST" as "(%st_srcL & %st_tgtL & %st_srcR & %st_tgtR & (#-> & #->) & IST)".
-    iDestruct "IST" as "((% & IST) & #->)". unfold Ist. rename H2 into INCL.
-    iDestruct "IST" as "(%l_tgt & %l_src & (#-> & #-> & %LEN) & (ACTIVATED & FREE & UNACTIVATED))".
-    steps_l. hss. rename q2 into l_src. iDestruct "ASM" as "(_ & #<-)". hss.
-    steps_r. hss. steps_r. inline_r. steps_r. do 3 force_r.
-    instantiate (1 := (_, SingleCoinPrT.t)). ss.
-    iPoseProof (free_from_split with "FREE") as "[FREE ARG]". iSplitL "ARG".
-    { iSplit; ss. iSplit; ss. rewrite LEN. et. }
-    steps_r. iDestruct "GRT" as "((%b & #-> & P) & _)". hss. steps_r.
-    iEval (rewrite LEN) in "P".
-    iPoseProof (initialized_update with "ACTIVATED") as "D"; et.
-    iPoseProof ("D" with "UNACTIVATED") as "D".
-    iPoseProof ("D" with "P") as "D". iApply isim_upd. iMod "D" as "[ACTIVATED UNACTIVATED]".
-    iModIntro. Local Opaque initialized_until.
-    force_l. instantiate (1 := b). steps_l. hss. do 2 force_l.
-    iPoseProof (initialized_until_readable with "ACTIVATED") as "[ACTIVATED POST]".
-    iSplitL "POST". { iSplit; ss. et. }
-    step. iSplit; et. iExists [_],[_],_,_. iSplit; et.
-    iSplit; et. iSplit; et. iExists _,_. iSplit; ss.
-    { iPureIntro. splits; et. rewrite !app_length. ss. nia. }
-    rewrite app_length. ss. rewrite plus_comm. ss. iFrame.
-  Qed.
-
-  Lemma simF_read:
-    HSim.sim_fun SingleCoinAMod SingleCoinPMod IstFull SingleCoinName.read.
-  Proof.
-    init_simF. unfold IstFull, IstProd0.
-    iDestruct "IST" as "(%st_srcL & %st_tgtL & %st_srcR & %st_tgtR & (#-> & #->) & IST)".
-    iDestruct "IST" as "((% & IST) & #->)". unfold Ist. rename H2 into INCL.
-    iDestruct "IST" as "(%l_tgt & %l_src & (#-> & #-> & %LEN) & (ACTIVATED & FREE & UNACTIVATED))".
-    steps_l. hss. rename q2 into l_src. iDestruct "ASM" as "((% & R) & %)". hss.
-    steps_r. hss. steps_r. iPoseProof (uninitialized_readable_disjoint with "UNACTIVATED R") as "%ran".
-    destruct nth_error eqn: E. 2:{ rewrite nth_error_None in E. nia. }
-    destruct (nth_error l_tgt) eqn: E0. 2:{ rewrite nth_error_None in E0. nia. }
-    destruct o.
-    - iPoseProof (initialized_until_same with "ACTIVATED") as "%"; et.
-      steps_r. steps_l. do 2 force_l. iFrame. iSplit; et. step.
-      iSplit; et. iExists [_],[_],_,_. iSplit; et.
-      iSplit; et. iSplit; et. iExists _,_. iSplit; ss. iFrame.
-    - steps_r. hss. iPoseProof (initialized_until_update_proph with "ACTIVATED") as "[A (%nth & P)]"; et.
-      inline_r. steps_r. do 3 force_r.
-      instantiate (1 := (_,_, existT _ (_,_,_))). ss. iSplitL "P". { iSplit; ss. iSplit; ss. ss. }
-      steps_r. iDestruct "GRT" as "((% & P) & _)". hss. steps_r. steps_l. do 2 force_l.
-      iFrame. iSplit; et. step. inv H3. 2:{ exfalso. apply NIN. econs. }
-      iSplit; et. iExists [_],[_],_,_. iSplit; et.
-      iSplit; et. iSplit; et. iExists _,_. iSplit; ss; iFrame.
-      iPureIntro. splits; et. rewrite <- (take_drop (S q) l_src).
-      rewrite !app_length. ss. rewrite !take_length. rewrite !drop_length. nia.
-  Qed.
-
-  Theorem sim:
-    HSim.t SingleCoinAMod SingleCoinPMod SingleCoinA.InitCond IstFull.
-  Proof.
-    init_sim.
-    - iIntros "A". iExists _,_,[],[]. iSplit.
-      { rewrite !app_nil_r. eauto. }
-      iSplit; [iSplit|]; eauto. iExists _,_. iSplit; et.
-    - eapply simF_new; eauto.
-    - eapply simF_read; eauto.
-  Qed.
-
-End SIMMODSEM.
-End SingleCoinPA. *)
