single_coin/SingleCoinIPproof.v
@@ -1,0 +1,54 @@
+Require Import CRIS CallFilter.
+Require Export SingleCoinHeader SingleCoinI SingleCoinP.
+Require Export ProphecyHeader ProphecyI.
+
+Module SingleCoinIP. Section SingleCoinIP.
+  Import SingleCoinP SingleCoinI.
+  Context `{!crisG Γ Σ α β τ _S _I, !concGS}.
+  Context (mn : string).
+
+  Local Notation MA := (SingleCoinP.t mn ★ ProphecyI.t mn).
+  Local Notation MI := (CFilter.filter (ProphecyName.exports mn) SingleCoinI.t ★ ProphecyI.t mn).
+
+  Local Definition Ist : ist_type Σ :=
+    (λ st_s st_t,
+      ∃ (l : list (option bool)), ⌜st_s = {[v_coins := Some l↑]} ∧ st_t = st_s⌝)%I.
+
+  Local Definition IstFull := IstProd (IstSB (Mod.scopes (SingleCoinP.t mn)) Ist) IstEq.
+
+  Lemma simF_new : ISim.sim_fun open MA MI IstFull (Some SingleCoinHdr.new).
+  Proof.
+    iStartSim.
+    iDestruct "IST" as "%"; des; subst.
+    steps_l. steps_r. destruct Any.downcast; steps_l; last case_match; steps_l; ss.
+    steps_r. inline_l. rewrite /ProphecyI.new. steps_l. step.
+    iSplit; eauto. do 4 iExists _. iSplit; eauto.
+    do 2 (iSplit; eauto; ss).
+  Qed.
+
+  Lemma simF_read : ISim.sim_fun open MA MI IstFull (Some SingleCoinHdr.read).
+  Proof.
+    iStartSim.
+    iDestruct "IST" as "%"; des; subst.
+    steps_l. steps_r. destruct (Any.downcast arg); steps_l; last case_match; steps_l; ss.
+    steps_r. des_ifs.
+    { step; eauto. iSplit; eauto.
+      do 4 iExists _. iSplit; eauto; cycle 1.
+      do 2 (iSplit; eauto; ss).
+    }
+    { steps_r. force_l. steps_l. rewrite /v_coins /SingleCoinP.v_coins.
+      inline_l. rewrite /ProphecyI.new. steps_l. step. iSplit; eauto.
+      do 4 iExists _. iSplit; eauto.
+      do 2 (iSplit; eauto; ss).
+    }
+    { rewrite /triggerUB. steps_l. des_ifs; steps_l; ss. }
+  Qed.
+
+  Lemma sim : ISim.t open MA MI emp%I IstFull.
+  Proof.
+    init_sim.
+    { eapply simF_new; eauto. }
+    { eapply simF_read; eauto. }
+    { iPureIntro; esplits; ss. }
+  Qed.
+End SingleCoinIP. End SingleCoinIP.
